FromAxioms/Algebra.lean
@@ -13,3 +13,5 @@ import FromAxioms.Algebra.Group
 import FromAxioms.Algebra.FinProd
 import FromAxioms.Algebra.Ring
 import FromAxioms.Algebra.Field
+import FromAxioms.Algebra.Poly
+import FromAxioms.Algebra.PolyRing
